xtext/org.archware.sosadl/src/org/archware/sosadl/validation/typing/proof/Incrementally_cons.java
@@ -2,17 +2,12 @@ package org.archware.sosadl.validation.typing.proof;
 
 import java.util.List;
 
-import org.archware.sosadl.validation.typing.EnvContent;
 import org.archware.sosadl.validation.typing.Environment;
 
 public class Incrementally_cons<T,P> implements Incrementally<T,P> {
 	@Mandatory private final Environment gamma;
 	
 	@Mandatory private final T x;
-	
-	private final String n;
-	
-	private final EnvContent c;
 	
 	@Mandatory private final Environment gammai;
 	
@@ -22,29 +17,18 @@ public class Incrementally_cons<T,P> implements Incrementally<T,P> {
 	
 	@Mandatory private final P p1;
 	
-	@Mandatory private final Equality p2;
+	@Mandatory private final Incrementally<T,P> p2;
 
-	@Mandatory private final Equality p3;
-
-	@Mandatory private final Equality p4;
-
-	@Mandatory private final Incrementally<T,P> p5;
-
-	public Incrementally_cons(Environment gamma, T x, String n, EnvContent c, Environment gammai, List<T> l,
-			Environment gamma1, P p1, Equality p2, Equality p3, Equality p4, Incrementally<T, P> p5) {
+	public Incrementally_cons(Environment gamma, T x, Environment gammai, List<T> l,
+			Environment gamma1, P p1, Incrementally<T, P> p2) {
 		super();
 		this.gamma = gamma;
 		this.x = x;
-		this.n = n;
-		this.c = c;
 		this.gammai = gammai;
 		this.l = l;
 		this.gamma1 = gamma1;
 		this.p1 = p1;
 		this.p2 = p2;
-		this.p3 = p3;
-		this.p4 = p4;
-		this.p5 = p5;
 	}
 
 	public Environment getGamma() {
@@ -53,14 +37,6 @@ public class Incrementally_cons<T,P> implements Incrementally<T,P> {
 
 	public T getX() {
 		return x;
-	}
-
-	public String getN() {
-		return n;
-	}
-
-	public EnvContent getC() {
-		return c;
 	}
 
 	public Environment getGammai() {
@@ -79,20 +55,8 @@ public class Incrementally_cons<T,P> implements Incrementally<T,P> {
 		return p1;
 	}
 
-	public Equality getP2() {
+	public Incrementally<T, P> getP2() {
 		return p2;
-	}
-
-	public Equality getP3() {
-		return p3;
-	}
-
-	public Equality getP4() {
-		return p4;
-	}
-
-	public Incrementally<T, P> getP5() {
-		return p5;
 	}
 
 }
